cedar-lean/Cedar/Thm/Validation/UpdateSchema.lean
@@ -8,147 +8,111 @@ open Cedar.Data
 open Cedar.Spec
 open Cedar.Validation
 
-/-- a schema is well formed if the entity and action type stores are well formed maps,
-and any uid present in the action type store is not present in the entity type store.
-the last assumption is true of generated schemas, and having it explicitly be a
-pre-condition makes proofs a bit easier (i think) (i might be wrong in which case
-it is a fairly simple refactor).
+/-!
+This file proves properties about the `updateSchema` utility function.
 -/
-def wf_schema (schema : Schema) : Prop :=
-Map.WellFormed schema.ets ∧ Map.WellFormed schema.acts
-∧ (∀ k ∈ schema.acts, k.ty ∉ schema.ets)
 
-/-- this theorem states that `updateSchema` adds an entry to the entity type store,
-that is consistent with its associated action type store entry. -/
-def updateSchemaPreservesEntityTypes (schema newSchema : Schema) :
-  wf_schema schema →
-  newSchema = updateSchema schema →
-  (∀ uid actsEntry, schema.acts.find? uid = some actsEntry →
-  ∃ etsEntry, newSchema.ets.find? uid.ty = some etsEntry ∧
-  ∀ ancestor ∈ actsEntry.ancestors, ancestor.ty ∈ etsEntry.ancestors)
-:= by
-  simp only [wf_schema, and_imp]
-  intro wfe₀ _ _ h₀ uid actsEntry h₁
-  simp only [updateSchema] at h₀
-  exists Prod.snd <| updateSchema.makeEntitySchemaEntries uid.ty (schema.acts.mapOnValues actionSchemaEntryToEntityData)
-  constructor
-  case left =>
-    simp only [h₀]
-    generalize h₂ : (updateSchema.makeEntitySchemaEntries uid.ty (Map.mapOnValues actionSchemaEntryToEntityData schema.acts)) = etsPair
-    have ⟨ety, etsEntry⟩ := etsPair
-    simp only
-    generalize h₃ : (List.map
-          (fun x => updateSchema.makeEntitySchemaEntries x (Map.mapOnValues actionSchemaEntryToEntityData schema.acts))
-          (Set.make
-              (Set.map (fun x => x.ty) (Map.mapOnValues actionSchemaEntryToEntityData schema.acts).keys).elts).elts) = m₀
-    rw [← Map.in_list_iff_find?_some]
-    apply Map.mem_append
-    have h₄ : uid.ty = ety := by
-      simp only [updateSchema.makeEntitySchemaEntries, Prod.mk.injEq] at h₂
-      simp only [h₂]
-    subst h₄
-    right
-    have h₄ : uid ∈ (Map.mapOnValues actionSchemaEntryToEntityData schema.acts).keys := by
-      rw [Map.keys_mapOnValues]
-      have h₅ := Map.find?_mem_toList h₁
-      simp only [Map.toList] at h₅
-      simp only [Map.in_list_in_keys h₅]
-    have h₅ : uid.ty ∈ ((Set.map (fun x => x.ty) (Map.mapOnValues actionSchemaEntryToEntityData schema.acts).keys)) := by
-      simp only [Set.map]
-      rw [← Set.make_mem]
-      simp only [Set.elts, List.mem_map]
-      exists uid
-    have ⟨h₆, _⟩ := Set.make_mem uid.ty (Set.map (fun x => x.ty) (Map.mapOnValues actionSchemaEntryToEntityData schema.acts).keys).elts
-    rw [← Set.in_list_iff_in_set] at h₅
-    simp only [h₅, true_implies] at h₆
-    rw [← Set.in_list_iff_in_set] at h₆
-    generalize h₇ : (fun x => updateSchema.makeEntitySchemaEntries x (Map.mapOnValues actionSchemaEntryToEntityData schema.acts)) = f at *
-    generalize h₈ : (Set.make (Set.map (fun x => x.ty) (Map.mapOnValues actionSchemaEntryToEntityData schema.acts).keys).elts) = s at *
-    have h₉ := List.mem_map_of_mem f h₆
-    rw [h₃] at h₉
-    rw [← h₇] at h₉
-    simp only at h₉
-    rw [h₂] at h₉
-    apply Map.mem_list_mem_make
-    have h₁₀ : Set.WellFormed s := by
-      subst h₈
-      simp only [Set.make_wf]
-    rw [Set.wf_iff_sorted] at h₁₀
-    simp only [List.Sorted] at h₁₀
-    subst h₃
-    have h₁₂ : List.SortedBy id (List.map Prod.fst (List.map f s.elts)) := by
-      simp only [List.map_map]
-      subst h₇
-      simp only [updateSchema.makeEntitySchemaEntries]
-      unfold Function.comp
-      simp only [List.map_id']
-      exact h₁₀
-    apply List.map_sortedBy_id
-    exact h₁₂
-    exact h₉
-    have h₄ : Map.WellFormed (Map.make m₀) := by simp [Map.make_wf m₀]
-    apply Map.wf_append wfe₀ h₄
-  case right =>
-    intro ancestor ain
-    simp only [updateSchema.makeEntitySchemaEntries]
-    have h₂ := Map.find?_mem_toList h₁
-    have h₃ : actionSchemaEntryToEntityData actsEntry ∈ (Map.filter (fun k _ => k.ty == uid.ty)
-            (Map.mapOnValues actionSchemaEntryToEntityData schema.acts)).values := by
-      simp only [Map.values, Map.filter, List.mem_map]
-      exists (uid, actionSchemaEntryToEntityData actsEntry)
-      constructor
-      rw [List.mem_filter]
-      constructor
-      simp only [Map.toList] at h₂
-      simp only [Map.in_kvs_in_mapOnValues h₂]
-      simp only [beq_self_eq_true]
-      simp only
-    rw [← Set.make_mem, List.mem_join]
-    exists (List.map (fun x => x.ty) (actionSchemaEntryToEntityData actsEntry).ancestors.elts)
-    simp only [List.mem_map]
-    constructor
-    exists actionSchemaEntryToEntityData actsEntry
-    exists ancestor
+/-- `updateSchema` does not modify the action part of the schema. -/
+def update_schema_preserves_action_schema (schema : Schema) :
+  (updateSchema schema).acts = schema.acts
+:= by simp only [updateSchema]
 
--- this theorem states that updateSchema does not modify the action type store.
-def updateSchemaPreservesActionSchema (schema newSchema : Schema) :
-  newSchema = updateSchema schema →
-  newSchema.acts = schema.acts
-:= by
-  intro h₀
-  simp only [updateSchema] at h₀
-  simp [h₀]
+/--
+In order to apply `updateSchema` safely, no actions types should be defined in
+entity type store. We expect the Rust code to produce schemas that satisfy this
+requirement.
 
-/-- for every entry in the entity type store of the updated schema, it is either an entry in the entity type store of the original schema, or there exists some uid such that its type matches the entry, and it has an entry in the action type store of the original schema. note that there can be multiple uids that have the same type, we only want to prove that one exists.
+(Technically, we could be more flexible here and say that re-definition is allowed
+as long as the two definitions are consistent, but that generalization is not
+needed at the moment.)
 -/
-def updateSchemaProducesWellFormedEntitySchema (schema newSchema : Schema) :
-  newSchema = updateSchema schema →
-  (∀ ty etsEntry, newSchema.ets.find? ty = some etsEntry →
-  schema.ets.find? ty = some etsEntry ∨
-  (schema.ets.find? ty = none ∧ ∃ uid actsEntry, uid.ty = ty ∧ schema.acts.find? uid = some actsEntry))
+def NoActionTypesInETS (schema : Schema) : Prop :=
+  ∀ uid ∈ schema.acts, uid.ty ∉ schema.ets
+
+def EntriesMatch (actsEntry: EntityUID × ActionSchemaEntry) (etsEntry: EntityType × EntitySchemaEntry) : Prop :=
+  actsEntry.1.ty = etsEntry.1 ∧ ∀ ancestor ∈ actsEntry.2.ancestors, ancestor.ty ∈ etsEntry.2.ancestors
+
+def mem_action_schema_to_entity_schema (acts : ActionSchema) :
+  ∀ ty etsEntry, (ty, etsEntry) ∈ (actionSchemaToEntitySchema acts).kvs →
+  ∃ uid actsEntry, (uid, actsEntry) ∈ acts.kvs ∧ EntriesMatch (uid, actsEntry) (ty, etsEntry)
+:= by
+  intro ty etsEntry h₀
+  simp only [actionSchemaToEntitySchema] at h₀
+  replace h₀ := Map.make_mem_list_mem h₀
+  -- TODO
+  sorry
+
+def no_action_types_in_ets_implies_disjoint (schema : Schema) :
+  NoActionTypesInETS schema →
+  schema.ets.Disjoint (actionSchemaToEntitySchema schema.acts)
+:= by
+   -- TODO
+   sorry
+
+/--
+`updateSchema` preserves existing entity types in the schema, assuming there
+is no overlap with the action types.
+-/
+def update_schema_preserves_entity_types (schema : Schema) :
+  NoActionTypesInETS schema →
+  ∀ ty etsEntry, (ty, etsEntry) ∈ schema.ets.kvs →
+  (ty, etsEntry) ∈ (updateSchema schema).ets.kvs
 := by
   intro h₀ ty etsEntry h₁
-  cases h₂ : Map.find? schema.ets ty with
-  | none =>
+  simp only [updateSchema]
+  apply Map.mem_append_converse
+  apply no_action_types_in_ets_implies_disjoint
+  assumption
+  left
+  assumption
+
+/--
+`updateSchema` adds an appropriate entity type for every action, assuming there
+is no overlap between entity and action types.
+-/
+def update_schema_adds_action_entity_types (schema : Schema) :
+  NoActionTypesInETS schema →
+  ∀ uid actsEntry, (uid, actsEntry) ∈ schema.acts.kvs →
+  ∃ ty etsEntry, (ty, etsEntry) ∈ (updateSchema schema).ets.kvs ∧
+  EntriesMatch (uid, actsEntry) (ty, etsEntry)
+:= by
+  intro h₀ uid actsEntry h₁
+  simp only [updateSchema]
+  exists uid.ty
+  exists Prod.snd (makeEntitySchemaEntry uid.ty (schema.acts.mapOnValues actionSchemaEntryToEntityData))
+  constructor
+  case left =>
+    generalize h₂ : (makeEntitySchemaEntry uid.ty (schema.acts.mapOnValues actionSchemaEntryToEntityData)) = etsPair
+    replace ⟨ety, etsEntry⟩ := etsPair
+    simp only
+    apply Map.mem_append_converse
+    apply no_action_types_in_ets_implies_disjoint
+    assumption
     right
-    constructor
-    rfl
+    -- TODO
     sorry
-  | some val =>
-    left
-    simp only [Option.some.injEq]
-    simp only [updateSchema, updateSchema.makeEntitySchemaEntries] at h₀
-    generalize h₃ : Map.make
-          (List.map
-            (fun x =>
-              (x,
-                {
-                  ancestors :=
-                    Set.make
-                      (List.map (fun edt => List.map (fun x => x.ty) edt.ancestors.elts)
-                          (Map.filter (fun k x_1 => k.ty == x)
-                              (Map.mapOnValues actionSchemaEntryToEntityData schema.acts)).values).join,
-                  attrs := Map.empty } ) : EntityType → EntityType × EntitySchemaEntry)
-            (Set.make
-                (Set.map (fun x => x.ty) (Map.mapOnValues actionSchemaEntryToEntityData schema.acts).keys).elts).elts) = m₀ at *
+  case right =>
+    -- TODO
     sorry
+
+/--
+`updateSchema` doesn't add any new entity type entries, beyond what is covered
+by `update_schema_preserves_entity_types` and `update_schema_adds_action_entities`.
+I.e. every entity type in the updated schema is either a type from the original
+schema, or there exists some action with that type.
+-/
+def update_schema_does_not_add_extra_types (schema : Schema) :
+  ∀ ty etsEntry, (ty, etsEntry) ∈ (updateSchema schema).ets.kvs →
+  (ty, etsEntry) ∈ schema.ets.kvs ∨
+  ∃ uid actsEntry, (uid, actsEntry) ∈ schema.acts.kvs ∧ EntriesMatch (uid, actsEntry) (ty, etsEntry)
+:= by
+  intro ty etsEntry h₀
+  simp only [updateSchema] at h₀
+  replace h₀ := Map.mem_append _ _ _ _ h₀
+  cases h₀
+  left
+  assumption
+  rename_i h₁
+  right
+  apply mem_action_schema_to_entity_schema
+  assumption
